Update seq.dfy

seq.dfy
@@ -1,50 +1,43 @@
+predicate esteSolutieValida(solutie : seq<int>)
+{
+  |solutie| == 4 && solutie[0]>=0 && solutie[1]>=0 && solutie[2]>=0 && solutie[3]>=0
+}
+
+
+
 predicate esteSolutie(solutie : seq<int>, nr:int)
-   requires |solutie| == 4
-   requires solutie[0]>=0
-   requires solutie[1]>=0
-   requires solutie[2]>=0
-   requires solutie[3]>=0
+  requires esteSolutieValida(solutie)
 {
     solutie[0]*1+solutie[1]*5+solutie[2]*10+solutie[3]*20 == nr
 
 }
 
+
 function cost(solutie : seq<int>):int 
-   requires |solutie| == 4
-   requires solutie[0]>=0
-   requires solutie[1]>=0
-   requires solutie[2]>=0
-   requires solutie[3]>=0
+  requires esteSolutieValida(solutie)
 {
     solutie[0]+solutie[1]+solutie[2]+solutie[3]
 }
 
 predicate esteSolutieOptima(solutie : seq<int>, nr:int)
-    requires |solutie| == 4
-    requires solutie[0]>=0
-    requires solutie[1]>=0
-    requires solutie[2]>=0
-    requires solutie[3]>=0
+    requires esteSolutieValida(solutie)
 {   
   esteSolutie(solutie,nr) &&
-  forall solutieOarecare :: |solutieOarecare| == 4 && solutieOarecare[0]>=0 && solutieOarecare[1]>=0 
-        && solutieOarecare[2]>=0 && solutieOarecare[3]>=0 && esteSolutie(solutieOarecare,nr) 
+  forall solutieOarecare :: esteSolutieValida(solutieOarecare) && esteSolutie(solutieOarecare,nr) 
           ==> cost(solutieOarecare) >= cost(solutie)
 
 }
 
 predicate INV(copie: int, nr: int, solutieFinala : seq<int>)
-  requires |solutieFinala| == 4
-  requires solutieFinala[0] >= 0
-  requires solutieFinala[1] >= 0
-  requires solutieFinala[2] >= 0
-  requires solutieFinala[3] >= 0
+  requires esteSolutieValida(solutieFinala)
 {
-   forall solutieCurenta :: |solutieCurenta| == 4 && solutieCurenta[0] >= 0 && solutieCurenta[1] >=0 && solutieCurenta[2]>=0 && solutieCurenta[3] >= 0 ==>
+   forall solutieCurenta :: esteSolutieValida(solutieCurenta) ==>
           (esteSolutie(solutieCurenta,copie) ==> 
-          esteSolutie([solutieFinala[0]+solutieCurenta[0],solutieFinala[1]+solutieCurenta[1],solutieFinala[2]+solutieCurenta[2],solutieFinala[3]+solutieCurenta[3]],nr)) &&
+          esteSolutie([solutieFinala[0]+solutieCurenta[0],solutieFinala[1]+solutieCurenta[1],
+          solutieFinala[2]+solutieCurenta[2],solutieFinala[3]+solutieCurenta[3]],nr)) &&
           (esteSolutieOptima(solutieCurenta,copie) ==> 
-          esteSolutieOptima([solutieFinala[0]+solutieCurenta[0],solutieFinala[1]+solutieCurenta[1],solutieFinala[2]+solutieCurenta[2],solutieFinala[3]+solutieCurenta[3]],nr))
+          esteSolutieOptima([solutieFinala[0]+solutieCurenta[0],solutieFinala[1]+solutieCurenta[1],
+          solutieFinala[2]+solutieCurenta[2],solutieFinala[3]+solutieCurenta[3]],nr))
 }
 
 
@@ -76,37 +69,30 @@ method gasireMaxim(nr: int) returns(s:int)
 
 lemma cazMaxim1(copie: int, nr: int, solutieFinala: seq<int>)
   requires copie < 5
-  requires |solutieFinala| == 4
-  requires solutieFinala[0] >= 0
-  requires solutieFinala[1] >= 0
-  requires solutieFinala[2] >= 0
-  requires solutieFinala[3] >= 0
+  requires esteSolutieValida(solutieFinala)
   requires INV(copie,nr,solutieFinala)
   ensures INV(copie-1,nr,[(solutieFinala[0]+1),solutieFinala[1],solutieFinala[2],solutieFinala[3]])
 {
 
-  forall solutieCurenta | |solutieCurenta| == 4 && solutieCurenta[0] >= 0 && solutieCurenta[1] >=0 
-          && solutieCurenta[2] >= 0  && solutieCurenta[3]>=0 && esteSolutieOptima(solutieCurenta,copie-1) 
+  forall solutieCurenta | esteSolutieValida(solutieCurenta) && esteSolutieOptima(solutieCurenta,copie-1) 
           ensures esteSolutieOptima([solutieFinala[0]+solutieCurenta[0]+1,solutieFinala[1]+solutieCurenta[1],
           solutieFinala[2]+solutieCurenta[2],solutieFinala[3]+solutieCurenta[3]],nr)
   {
     assert esteSolutie(solutieCurenta,copie-1);
     assert esteSolutie([solutieCurenta[0]+1,solutieCurenta[1],solutieCurenta[2],solutieCurenta[3]],copie);
 
-    assert forall solutieOarecare :: |solutieOarecare| == 4 && solutieOarecare[0]>=0 && solutieOarecare[1]>=0 
-          && solutieOarecare[2]>=0 && solutieOarecare[3]>=0 && esteSolutie(solutieOarecare,copie-1) 
+    assert forall solutieOarecare :: esteSolutieValida(solutieOarecare) && esteSolutie(solutieOarecare,copie-1) 
           ==> cost(solutieOarecare) >= cost(solutieCurenta);
 
     assert esteSolutie([solutieFinala[0]+solutieCurenta[0]+1,solutieFinala[1]+solutieCurenta[1],
           solutieFinala[2]+solutieCurenta[2],solutieFinala[3]+solutieCurenta[3]],nr);
 
-    assert forall solutieOarecare :: |solutieOarecare| == 4 && solutieOarecare[0]>=0 && solutieOarecare[1]>=0 
-          && solutieOarecare[2]>=0 && solutieOarecare[3]>=0 &&  esteSolutie(solutieOarecare,nr) 
+    assert forall solutieOarecare :: esteSolutieValida(solutieOarecare) &&  esteSolutie(solutieOarecare,nr) 
           ==> cost(solutieOarecare) >= cost([solutieCurenta[0]+solutieFinala[0]+1,solutieCurenta[1]+solutieFinala[1],
           solutieCurenta[2]+solutieFinala[2],solutieCurenta[3]+solutieFinala[3]]);
   }
 
-  assert forall solutieCurenta :: |solutieCurenta|==4 && solutieCurenta[0]>=0 && solutieCurenta[1]>=0 && solutieCurenta[2]>=0 && solutieCurenta[3]>=0 
+  assert forall solutieCurenta :: esteSolutieValida(solutieCurenta) 
           && esteSolutieOptima(solutieCurenta,copie-1) ==> 
           esteSolutieOptima([solutieFinala[0]+solutieCurenta[0]+1,solutieFinala[1]+solutieCurenta[1],
           solutieFinala[2]+solutieCurenta[2],solutieFinala[3]+solutieCurenta[3]],nr);
@@ -115,72 +101,115 @@ lemma cazMaxim1(copie: int, nr: int, solutieFinala: seq<int>)
 
 lemma cazMaxim5(copie: int, nr: int, solutieFinala: seq<int>)
   requires 5 <= copie < 10 
-  requires |solutieFinala| == 4
-  requires solutieFinala[0] >= 0
-  requires solutieFinala[1] >= 0
-  requires solutieFinala[2] >= 0
-  requires solutieFinala[3] >= 0 
+  requires esteSolutieValida(solutieFinala)
   requires INV(copie,nr,solutieFinala)
   ensures INV(copie-5,nr,[solutieFinala[0],(solutieFinala[1]+1),solutieFinala[2],solutieFinala[3]])
 {
 
- forall solutieCurenta | |solutieCurenta| == 4 && solutieCurenta[0]>=0 && solutieCurenta[1]>=0 && 
-          solutieCurenta[2]>=0 && solutieCurenta[3]>=0 && esteSolutieOptima(solutieCurenta,copie-5) 
+ forall solutieCurenta | esteSolutieValida(solutieCurenta) && esteSolutieOptima(solutieCurenta,copie-5) 
           ensures esteSolutieOptima([solutieFinala[0]+solutieCurenta[0],solutieFinala[1]+solutieCurenta[1]+1,
           solutieCurenta[2]+solutieFinala[2],solutieCurenta[3]+solutieFinala[3]],nr)
   {
     assert esteSolutie(solutieCurenta,copie-5);
     assert esteSolutie([solutieCurenta[0], solutieCurenta[1]+1,solutieCurenta[2],solutieCurenta[3]],copie);
 
-    assert forall solutieOarecare :: |solutieOarecare| == 4 && solutieOarecare[0]>=0 && solutieOarecare[1]>=0 &&
-          solutieOarecare[2]>=0 && solutieOarecare[3]>=0  && esteSolutie(solutieOarecare,copie-5) 
+    assert forall solutieOarecare :: esteSolutieValida(solutieOarecare)  && esteSolutie(solutieOarecare,copie-5) 
           ==> cost(solutieOarecare) >= cost(solutieCurenta);
     assert esteSolutie([solutieFinala[0]+solutieCurenta[0],solutieFinala[1]+solutieCurenta[1]+1,solutieFinala[2]+solutieCurenta[2],solutieFinala[3]+solutieCurenta[3]],nr);
     
-    assert forall solutieOarecare :: |solutieOarecare| == 4 && solutieOarecare[0]>=0 && solutieOarecare[1]>=0 && solutieOarecare[2]>=0 
-          && solutieOarecare[3]>=0 && esteSolutie(solutieOarecare,nr)
+    assert forall solutieOarecare :: esteSolutieValida(solutieOarecare) && esteSolutie(solutieOarecare,nr)
           ==> cost(solutieOarecare) >= cost([solutieFinala[0]+solutieCurenta[0],solutieFinala[1]+solutieCurenta[1]+1,solutieFinala[2]+solutieCurenta[2],solutieFinala[3]+solutieCurenta[3]]);
   }
 
-  assert forall solutieCurenta :: |solutieCurenta| == 4 && solutieCurenta[0]>=0 && solutieCurenta[1]>=0 && solutieCurenta[2]>=0
-          && solutieCurenta[3]>=0 && esteSolutie(solutieCurenta,copie-5) ==> 
+  assert forall solutieCurenta :: esteSolutieValida(solutieCurenta) && esteSolutie(solutieCurenta,copie-5) ==> 
           esteSolutieOptima([solutieCurenta[0]+solutieFinala[0],solutieCurenta[1]+solutieFinala[1]+1,solutieCurenta[2]+solutieFinala[2],solutieCurenta[3]+solutieFinala[3]],nr);
 
 }
 
+lemma aux2(copie:int,solutieCurenta:seq<int>)
+  requires 10 <= copie < 20
+  requires esteSolutieValida(solutieCurenta)
+  requires esteSolutieOptima(solutieCurenta,copie-10)
+  ensures esteSolutieOptima([solutieCurenta[0], solutieCurenta[1],solutieCurenta[2]+1,solutieCurenta[3]],copie)
+{
+
+    assert esteSolutie([solutieCurenta[0], solutieCurenta[1],solutieCurenta[2]+1,solutieCurenta[3]],copie);
+    if(!esteSolutieOptima([solutieCurenta[0], solutieCurenta[1],solutieCurenta[2]+1,solutieCurenta[3]],copie))
+    {
+      var solopt :|esteSolutieValida(solopt) && esteSolutie(solopt,copie) && cost(solopt)<cost([solutieCurenta[0], solutieCurenta[1],solutieCurenta[2]+1,solutieCurenta[3]]);
+      assert cost([solutieCurenta[0], solutieCurenta[1],solutieCurenta[2]+1,solutieCurenta[3]]) == cost(solutieCurenta)+1;
+      assert solopt[3]==0;
+      if(solopt[2]>=1)
+      {
+        var solopt' := [solopt[0],solopt[1],solopt[2]-1,solopt[3]];
+        assert esteSolutie(solopt',copie-10);
+        assert cost(solopt') == cost(solopt)-1;
+        assert cost(solopt)-1 < cost(solutieCurenta);
+        assert false;
+      }
+      else if(solopt[1]>=2)
+      {
+        var solopt' := [solopt[0],solopt[1]-2,solopt[2],solopt[3]];
+        assert esteSolutie(solopt',copie-10);
+        assert cost(solopt') == cost(solopt)-2;
+        assert cost(solopt)-2 < cost(solutieCurenta);
+        assert false;
+      }else if(solopt[1]>=1 && solopt[0]>=5 )
+      {
+        var solopt' := [solopt[0]-5,solopt[1]-1,solopt[2],solopt[3]];
+        assert esteSolutie(solopt',copie-10);
+        assert cost(solopt') == cost(solopt)-6;
+        assert cost(solopt)-6 < cost(solutieCurenta);
+        assert false;
+      }
+      else if(solopt[0]>=10 )
+      {
+        var solopt' := [solopt[0]-10,solopt[1],solopt[2],solopt[3]];
+        assert esteSolutie(solopt',copie-10);
+        assert cost(solopt') == cost(solopt)-10;
+        assert cost(solopt)-10 < cost(solutieCurenta);
+        assert false;
+      }
+      else{
+        assert false;
+      }
+
+    }
+
+}
+
+
+
 lemma cazMaxim10(copie: int, nr: int, solutieFinala: seq<int>)
   requires 10 <= copie < 20 
-  requires |solutieFinala| == 4
-  requires solutieFinala[0] >= 0
-  requires solutieFinala[1] >= 0
-  requires solutieFinala[2] >= 0
-  requires solutieFinala[3] >= 0 
+  requires esteSolutieValida(solutieFinala) 
   requires INV(copie,nr,solutieFinala)
   ensures INV(copie-10,nr,[solutieFinala[0],solutieFinala[1],solutieFinala[2]+1,solutieFinala[3]])
 {
 
- forall solutieCurenta | |solutieCurenta| == 4 && solutieCurenta[0]>=0 && solutieCurenta[1]>=0 && 
-          solutieCurenta[2]>=0 && solutieCurenta[3]>=0 && esteSolutieOptima(solutieCurenta,copie-10) 
+ forall solutieCurenta | esteSolutieValida(solutieCurenta) && esteSolutieOptima(solutieCurenta,copie-10) 
           ensures esteSolutieOptima([solutieFinala[0]+solutieCurenta[0],solutieFinala[1]+solutieCurenta[1],
           solutieCurenta[2]+solutieFinala[2]+1,solutieCurenta[3]+solutieFinala[3]],nr)
   {
     assert esteSolutie(solutieCurenta,copie-10);
     assert esteSolutie([solutieCurenta[0], solutieCurenta[1],solutieCurenta[2]+1,solutieCurenta[3]],copie);
 
-    assert forall solutieOarecare :: |solutieOarecare| == 4 && solutieOarecare[0]>=0 && solutieOarecare[1]>=0 &&
-          solutieOarecare[2]>=0 && solutieOarecare[3]>=0  && esteSolutie(solutieOarecare,copie-10) 
+    aux2(copie,solutieCurenta);
+
+    assert esteSolutieOptima([solutieCurenta[0], solutieCurenta[1],solutieCurenta[2]+1,solutieCurenta[3]],copie);
+
+    assert forall solutieOarecare :: esteSolutieValida(solutieOarecare)  && esteSolutie(solutieOarecare,copie-10) 
           ==> cost(solutieOarecare) >= cost(solutieCurenta);
+    
 
     assert esteSolutie([solutieFinala[0]+solutieCurenta[0],solutieFinala[1]+solutieCurenta[1],1+solutieFinala[2]+solutieCurenta[2],solutieFinala[3]+solutieCurenta[3]],nr);
 
-    assert forall solutieOarecare :: |solutieOarecare| == 4 && solutieOarecare[0]>=0 && solutieOarecare[1]>=0 
-            && solutieOarecare[2]>=0 && solutieOarecare[3]>=0 && esteSolutie(solutieOarecare,nr)
+    assert forall solutieOarecare :: esteSolutieValida(solutieOarecare) && esteSolutie(solutieOarecare,nr)
           ==> cost(solutieOarecare) >= cost([solutieCurenta[0]+solutieFinala[0],solutieCurenta[1]+solutieFinala[1],
                                         solutieCurenta[2]+solutieFinala[2]+1,solutieCurenta[3]+solutieFinala[3]]);
   }
 
-  assert forall solutieCurenta :: |solutieCurenta| == 4 && solutieCurenta[0]>=0 && solutieCurenta[1]>=0 && solutieCurenta[2]>=0
-          && solutieCurenta[3]>=0 && esteSolutie(solutieCurenta,copie-10) ==> 
+  assert forall solutieCurenta :: esteSolutieValida(solutieCurenta) && esteSolutieOptima(solutieCurenta,copie-10) ==> 
           esteSolutieOptima([solutieCurenta[0]+solutieFinala[0],solutieCurenta[1]+solutieFinala[1],
                             solutieCurenta[2]+solutieFinala[2]+1,solutieCurenta[3]+solutieFinala[3]],nr);
 
@@ -189,16 +218,8 @@ lemma cazMaxim10(copie: int, nr: int, solutieFinala: seq<int>)
 
 
 lemma B(copie:int,nr: int,solutieOarecare : seq<int>, solutieCurenta: seq<int>)
-  requires |solutieOarecare| == 4
-  requires solutieOarecare[0]>=0
-  requires solutieOarecare[1]>=0
-  requires solutieOarecare[2]>=0
-  requires solutieOarecare[3]>=0
-  requires |solutieCurenta| == 4
-  requires solutieCurenta[0] >= 0
-  requires solutieCurenta[1] >= 0
-  requires solutieCurenta[2] >= 0
-  requires solutieCurenta[3] >= 0
+  requires esteSolutieValida(solutieOarecare)
+  requires esteSolutieValida(solutieCurenta)
   requires copie >= 20
   requires esteSolutie(solutieOarecare,copie)
   requires esteSolutie(solutieCurenta,copie-20)
@@ -222,40 +243,51 @@ lemma B(copie:int,nr: int,solutieOarecare : seq<int>, solutieCurenta: seq<int>)
       {
         assert (solutieOarecare[0]+(5*solutieOarecare[1])+(10*solutieOarecare[2]))>20;
         
-        if(solutieOarecare[0]>=20)
+        if(solutieOarecare[2]>=2)
         {
-          var nouaSolutieOarecare := [solutieOarecare[0]-20,solutieOarecare[1],solutieOarecare[2],solutieOarecare[3]+1];
-          B(copie,nr,nouaSolutieOarecare, solutieCurenta);
+            var nouaSolutieOarecare := [solutieOarecare[0],solutieOarecare[1],solutieOarecare[2]-2,solutieOarecare[3]+1];
+            B(copie,nr,nouaSolutieOarecare, solutieCurenta);
         }
-        else if(solutieOarecare[0]>=15 && solutieOarecare[1]>=1){
-               var nouaSolutieOarecare := [solutieOarecare[0]-15,solutieOarecare[1]-1,solutieOarecare[2],solutieOarecare[3]+1];
-                B(copie,nr,nouaSolutieOarecare, solutieCurenta);
+        else if(solutieOarecare[2]>=1 && solutieOarecare[1]>=2)
+        {
+            var nouaSolutieOarecare := [solutieOarecare[0],solutieOarecare[1]-2,solutieOarecare[2]-1,solutieOarecare[3]+1];
+            B(copie,nr,nouaSolutieOarecare, solutieCurenta);
         }
-        else if(solutieOarecare[0]>=10 && solutieOarecare[1]>=2){
-               var nouaSolutieOarecare := [solutieOarecare[0]-10,solutieOarecare[1]-2,solutieOarecare[2],solutieOarecare[3]+1];
-                B(copie,nr,nouaSolutieOarecare, solutieCurenta);
+        else if(solutieOarecare[2]>=1 && solutieOarecare[1]>=1 && solutieOarecare[0]>=5)
+        {
+            var nouaSolutieOarecare := [solutieOarecare[0]-5,solutieOarecare[1]-1,solutieOarecare[2]-1,solutieOarecare[3]+1];
+            B(copie,nr,nouaSolutieOarecare, solutieCurenta);
         }
-        else if(solutieOarecare[0]>=10 && solutieOarecare[2]>=1){
-               var nouaSolutieOarecare := [solutieOarecare[0]-10,solutieOarecare[1],solutieOarecare[2]-1,solutieOarecare[3]+1];
-                B(copie,nr,nouaSolutieOarecare, solutieCurenta);
+        else if(solutieOarecare[1]>=4)
+        {
+            var nouaSolutieOarecare := [solutieOarecare[0],solutieOarecare[1]-4,solutieOarecare[2],solutieOarecare[3]+1];
+            B(copie,nr,nouaSolutieOarecare, solutieCurenta);
         }
-        else if(solutieOarecare[0]>=5 && solutieOarecare[1]>=3){
-               var nouaSolutieOarecare := [solutieOarecare[0]-5,solutieOarecare[1]-3,solutieOarecare[2],solutieOarecare[3]+1];
-                B(copie,nr,nouaSolutieOarecare, solutieCurenta);
+        else if(solutieOarecare[1]>=3 && solutieOarecare[0]>=5)
+        {
+            var nouaSolutieOarecare := [solutieOarecare[0]-5,solutieOarecare[1]-3,solutieOarecare[2],solutieOarecare[3]+1];
+            B(copie,nr,nouaSolutieOarecare, solutieCurenta);
         }
-        else if(solutieOarecare[0]>=5 && solutieOarecare[1]>=1 && solutieOarecare[2]>=1){
-               var nouaSolutieOarecare := [solutieOarecare[0]-5,solutieOarecare[1]-1,solutieOarecare[2]-1,solutieOarecare[3]+1];
-                B(copie,nr,nouaSolutieOarecare, solutieCurenta);
+        else if(solutieOarecare[1]>=2 && solutieOarecare[0]>=10)
+        {
+            var nouaSolutieOarecare := [solutieOarecare[0]-10,solutieOarecare[1]-2,solutieOarecare[2],solutieOarecare[3]+1];
+            B(copie,nr,nouaSolutieOarecare, solutieCurenta);
         }
-        else if(solutieOarecare[1]>=2 && solutieOarecare[2]>=1){
-               var nouaSolutieOarecare := [solutieOarecare[0],solutieOarecare[1]-2,solutieOarecare[2]-1,solutieOarecare[3]+1];
-                B(copie,nr,nouaSolutieOarecare, solutieCurenta);
+        else if(solutieOarecare[1]>=1 && solutieOarecare[0]>=15)
+        {
+          var nouaSolutieOarecare := [solutieOarecare[0]-15,solutieOarecare[1]-1,solutieOarecare[2],solutieOarecare[3]+1];
+            B(copie,nr,nouaSolutieOarecare, solutieCurenta);
         }
-        else{
-               var nouaSolutieOarecare := [solutieOarecare[0],solutieOarecare[1],solutieOarecare[2]-2,solutieOarecare[3]+1];
-                B(copie,nr,nouaSolutieOarecare, solutieCurenta);
+        else if(solutieOarecare[0]>=20)
+        {
+            var nouaSolutieOarecare := [solutieOarecare[0]-20,solutieOarecare[1],solutieOarecare[2],solutieOarecare[3]+1];
+            B(copie,nr,nouaSolutieOarecare, solutieCurenta);
         }
-        
+        else if(solutieOarecare[2]>=1 && solutieOarecare[0]>=10)
+        {
+            var nouaSolutieOarecare := [solutieOarecare[0]-10,solutieOarecare[1],solutieOarecare[2]-1,solutieOarecare[3]+1];
+            B(copie,nr,nouaSolutieOarecare, solutieCurenta);
+        }
       }
 
     assert solutieOarecare[3] == (solutieCurenta[3]+1);
@@ -309,18 +341,13 @@ lemma B(copie:int,nr: int,solutieOarecare : seq<int>, solutieCurenta: seq<int>)
 }
 
 lemma esteSolutiePentruCopie(copie:int,nr: int, solutieCurenta:seq<int>)
-  requires |solutieCurenta| == 4
-  requires solutieCurenta[0] >= 0
-  requires solutieCurenta[1] >= 0
-  requires solutieCurenta[2] >= 0
-  requires solutieCurenta[3] >= 0
+  requires esteSolutieValida(solutieCurenta)
   requires copie >= 20
   requires esteSolutie(solutieCurenta,copie-20)
   requires esteSolutieOptima(solutieCurenta,copie-20)
   ensures esteSolutieOptima([solutieCurenta[0],solutieCurenta[1],solutieCurenta[2],1+solutieCurenta[3]],copie)
 {
-  forall solutieOarecare | |solutieOarecare| == 4 && solutieOarecare[0]>=0 && solutieOarecare[1]>=0 && 
-        solutieOarecare[2]>=0 && solutieOarecare[3]>=0 && esteSolutie(solutieOarecare,copie)
+  forall solutieOarecare | esteSolutieValida(solutieOarecare) && esteSolutie(solutieOarecare,copie)
     ensures cost(solutieOarecare)>=cost([solutieCurenta[0],solutieCurenta[1],solutieCurenta[2],1+solutieCurenta[3]])
   {
     B(copie,nr, solutieOarecare, solutieCurenta);
@@ -329,21 +356,9 @@ lemma esteSolutiePentruCopie(copie:int,nr: int, solutieCurenta:seq<int>)
 }
 
 lemma aux(copie: int ,nr: int, solutieOarecare : seq<int>, solutieFinala : seq<int>, solutieCurenta:seq<int>)
-  requires |solutieOarecare| == 4
-  requires solutieOarecare[0]>=0
-  requires solutieOarecare[1]>=0
-  requires solutieOarecare[2]>=0
-  requires solutieOarecare[3]>=0
-  requires |solutieFinala| == 4
-  requires solutieFinala[0] >= 0
-  requires solutieFinala[1] >= 0
-  requires solutieFinala[2] >= 0
-  requires solutieFinala[3] >= 0
-  requires |solutieCurenta| == 4
-  requires solutieCurenta[0] >= 0 
-  requires solutieCurenta[1] >= 0
-  requires solutieCurenta[2] >= 0
-  requires solutieCurenta[3] >= 0
+  requires esteSolutieValida(solutieOarecare)
+  requires esteSolutieValida(solutieFinala)
+  requires esteSolutieValida(solutieCurenta)
   requires copie >= 20
   requires esteSolutieOptima(solutieCurenta,copie-20)
   requires esteSolutie([solutieFinala[0]+solutieCurenta[0],solutieFinala[1]+solutieCurenta[1],solutieFinala[2]+solutieCurenta[2],1+solutieFinala[3]+solutieCurenta[3]],nr)
@@ -359,19 +374,15 @@ lemma aux(copie: int ,nr: int, solutieOarecare : seq<int>, solutieFinala : seq<i
 
 lemma cazMaxim20(copie: int,nr: int, solutieFinala : seq<int>)
   requires copie >= 20
-  requires |solutieFinala| == 4
-  requires solutieFinala[0] >= 0
-  requires solutieFinala[1] >= 0
-  requires solutieFinala[2] >= 0
-  requires solutieFinala[3] >= 0
+  requires esteSolutieValida(solutieFinala)
   requires INV(copie,nr,solutieFinala)
   ensures INV(copie-20,nr,[solutieFinala[0],solutieFinala[1],solutieFinala[2],solutieFinala[3]+1])
 {
-  assert forall solutieCurenta :: |solutieCurenta|==4  && solutieCurenta[0]>=0 && solutieCurenta[1]>=0 && solutieCurenta[2]>=0 && solutieCurenta[3]>=0 ==>
+  assert forall solutieCurenta :: esteSolutieValida(solutieCurenta) ==>
           (esteSolutie(solutieCurenta,copie) ==> 
           esteSolutie([solutieFinala[0]+solutieCurenta[0],solutieFinala[1]+solutieCurenta[1],solutieFinala[2]+solutieCurenta[2],solutieFinala[3]+solutieCurenta[3]],nr));
 
-   forall solutieCurenta | |solutieCurenta| == 4  && solutieCurenta[0]>=0 && solutieCurenta[1]>=0 && solutieCurenta[2]>=0 && solutieCurenta[3]>=0 
+   forall solutieCurenta | esteSolutieValida(solutieCurenta) 
           && esteSolutie(solutieCurenta,copie-20) 
           ensures esteSolutie([solutieFinala[0]+solutieCurenta[0],solutieFinala[1]+solutieCurenta[1],solutieFinala[2]+solutieCurenta[2],solutieFinala[3]+solutieCurenta[3]+1],nr)
    {
@@ -379,7 +390,7 @@ lemma cazMaxim20(copie: int,nr: int, solutieFinala : seq<int>)
    }
   
 
-  forall solutieCurenta | |solutieCurenta|==4 && solutieCurenta[0]>=0 && solutieCurenta[1]>=0 && solutieCurenta[2]>=0 && solutieCurenta[3]>=0 
+  forall solutieCurenta | esteSolutieValida(solutieCurenta) 
           && esteSolutieOptima(solutieCurenta,copie-20) 
           ensures esteSolutieOptima([solutieFinala[0]+solutieCurenta[0],solutieFinala[1]+solutieCurenta[1],solutieFinala[2]+solutieCurenta[2],solutieFinala[3]+solutieCurenta[3]+1],nr)
   {
@@ -387,36 +398,36 @@ lemma cazMaxim20(copie: int,nr: int, solutieFinala : seq<int>)
     assert esteSolutie(solutieCurenta,copie-20);
     assert esteSolutie([solutieCurenta[0],solutieCurenta[1],solutieCurenta[2],solutieCurenta[3]+1],copie);
 
-    assert forall solutieOarecare :: |solutieOarecare| == 4 && solutieOarecare[0]>=0 && solutieOarecare[1]>=0 && solutieOarecare[2]>=0 && solutieOarecare[3]>=0
+    assert forall solutieOarecare :: esteSolutieValida(solutieOarecare)
           && esteSolutie(solutieOarecare,copie-20) 
           ==> cost(solutieOarecare) >= cost(solutieCurenta);
 
 
     assert esteSolutie([solutieFinala[0]+solutieCurenta[0],solutieFinala[1]+solutieCurenta[1],solutieFinala[2]+solutieCurenta[2],solutieFinala[3]+solutieCurenta[3]+1],nr);
 
-    forall solutieOarecare | |solutieOarecare| == 4 && solutieOarecare[0]>=0 && solutieOarecare[1]>=0 && solutieOarecare[2]>=0 && solutieOarecare[3]>=0
+    forall solutieOarecare | esteSolutieValida(solutieOarecare)
                  && esteSolutie(solutieOarecare,nr)
       ensures cost(solutieOarecare) >= cost([solutieFinala[0]+solutieCurenta[0],solutieFinala[1]+solutieCurenta[1],solutieFinala[2]+solutieCurenta[2],1+solutieFinala[3]+solutieCurenta[3]])
       {
           aux(copie, nr, solutieOarecare, solutieFinala, solutieCurenta);
       }
 
-    assert forall solutieOarecare :: |solutieOarecare| == 4 && solutieOarecare[0]>=0 && solutieOarecare[1]>=0 && solutieOarecare[2]>=0 && solutieOarecare[3]>=0
+    assert forall solutieOarecare :: esteSolutieValida(solutieOarecare)
              && esteSolutie(solutieOarecare,nr) 
           ==> cost(solutieOarecare) >= cost([solutieFinala[0]+solutieCurenta[0],solutieFinala[1]+solutieCurenta[1],solutieFinala[2]+solutieCurenta[2],1+solutieFinala[3]+solutieCurenta[3]]);
   }
 
 
-  assert forall solutieCurenta :: |solutieCurenta| == 4 && solutieCurenta[0]>=0 && solutieCurenta[1]>=0 && solutieCurenta[2]>=0 && solutieCurenta[3]>=0
+  assert forall solutieCurenta :: esteSolutieValida(solutieCurenta)
           && esteSolutieOptima(solutieCurenta,copie-20) ==> 
           esteSolutieOptima([solutieFinala[0]+solutieCurenta[0],solutieFinala[1]+solutieCurenta[1],solutieFinala[2]+solutieCurenta[2],1+solutieFinala[3]+solutieCurenta[3]],nr);
 
 
-  assert forall solutieCurenta :: |solutieCurenta| == 4 && solutieCurenta[0]>=0 && solutieCurenta[1]>=0 && solutieCurenta[2]>=0 && solutieCurenta[3]>=0 ==>
+  assert forall solutieCurenta :: esteSolutieValida(solutieCurenta) ==>
           (esteSolutie(solutieCurenta,copie-20) ==> 
           esteSolutie([solutieFinala[0]+solutieCurenta[0],solutieFinala[1]+solutieCurenta[1],solutieFinala[2]+solutieCurenta[2],1+solutieFinala[3]+solutieCurenta[3]],nr));
   
-  assert forall solutieCurenta :: |solutieCurenta| == 4 && solutieCurenta[0]>=0 && solutieCurenta[1]>=0 && solutieCurenta[2]>=0 && solutieCurenta[3] >= 0 ==>        
+  assert forall solutieCurenta :: esteSolutieValida(solutieCurenta) ==>        
           (esteSolutieOptima(solutieCurenta,copie-20) ==> 
           esteSolutieOptima([solutieFinala[0]+solutieCurenta[0],solutieFinala[1]+solutieCurenta[1],solutieFinala[2]+solutieCurenta[2],solutieFinala[3]+solutieCurenta[3]+1],nr));
 
@@ -427,11 +438,7 @@ lemma cazMaxim20(copie: int,nr: int, solutieFinala : seq<int>)
 
   method nrMinimBancnote(nr: int) returns (solutie: seq<int>)
     requires nr>=0
-    ensures |solutie| == 4
-    ensures solutie[0]>=0
-    ensures solutie[1]>=0
-    ensures solutie[2]>=0
-    ensures solutie[3]>=0
+    ensures esteSolutieValida(solutie)
     ensures esteSolutie(solutie,nr)
     ensures esteSolutieOptima(solutie,nr)
 {
@@ -484,7 +491,7 @@ lemma cazMaxim20(copie: int,nr: int, solutieFinala : seq<int>)
 
 
 method Main() {
-  var nr:= 18;
+  var nr:= 58;
   var sol:=nrMinimBancnote(nr);
   print sol;
 }
